high2/Zeta.High.Verifier.EAC.fst
@@ -1,9 +1,11 @@
 module Zeta.High.Verifier.EAC
 
+open Zeta.BinTree
 open Zeta.Interleave
 open Zeta.App
 open Zeta.Key
 open Zeta.GenKey
+open Zeta.Merkle
 open Zeta.Record
 open Zeta.Time
 open Zeta.MultiSet
@@ -24,6 +26,7 @@ module GI=Zeta.Generic.Interleave
 module GB = Zeta.Generic.Blum
 module GTL=Zeta.Generic.TSLog
 module HI=Zeta.High.Interleave
+module HM = Zeta.High.Merkle
 module HTL=Zeta.High.TSLog
 
 noeq
@@ -105,13 +108,51 @@ let lemma_non_eac_init_addm
     lemma_addm_ancestor_is_proving itsli';
     assert(k' = proving_ancestor itsli k);
 
+    (* k' is in the verifier thread tid's cache before processing entry i *)
+    let st_pre = thread_store_pre tid itsl i in
+    assert(store_contains st_pre k');
 
+    let gk' = IntK #app k' in
+    eac_value_is_stored_value itsli gk' tid;
+    let mv' = HM.eac_value k' itsli in
+    let d = desc_dir k k' in
+    let dh' = desc_hash mv' d in
 
-    (* k' is in the verifier cache *)
-    //assert(store_contains (thread_store tid ))
+    lemma_proving_ancestor_initial itsli k;
 
+    match dh' with
+    | Empty -> hash_collision_contra app
+    | Desc k2 _ _ ->
+      lemma_desc_reflexive k;
+      hash_collision_contra app
 
-    admit()
+let lemma_non_eac_init_evict
+  (#app #n:_)
+  (itsl: neac_log app n
+    {let fi = eac_failure itsl in
+     fi.es = EACInit /\
+     is_evict fi.le})
+  : hash_collision app
+  = let fi = eac_failure itsl in
+    let i = fi.bi in
+    let k  = evict_slot fi.le in
+    let itsli = prefix itsl i in
+    let itsli' = prefix itsl (i+1) in
+    let tid = src itsl i in
+
+    // k is the verifier store prior to processing ...
+    let st_pre = thread_store tid itsli in
+    assert(store_contains st_pre k);
+
+    let aux ()
+      : Lemma (ensures (k <> Root))
+      = root_never_evicted itsl i
+    in
+    aux();
+
+    FStar.Classical.exists_intro (fun tid -> store_contains (thread_store tid itsli) k) tid;
+    lemma_instore k itsli;
+    hash_collision_contra app
 
 let lemma_neac_implies_hash_collision
   (#app #n:_)
@@ -125,8 +166,11 @@ let lemma_neac_implies_hash_collision
     | EACInit -> (
       match fi.le with
       | AddB _ _ _ _ -> lemma_non_eac_init_addb epmax itsl
-      | _ ->
-      admit()
+      | AddM _ _ _ -> lemma_non_eac_init_addm itsl
+      | EvictM _ _ -> lemma_non_eac_init_evict itsl
+      | EvictB _ _ -> lemma_non_eac_init_evict itsl
+      | EvictBM _ _ _ -> lemma_non_eac_init_evict itsl
+      | _ -> hash_collision_contra app
     )
     | _ ->
 
